ARMv8/ARMv8_Syntax.thy
@@ -1,5 +1,5 @@
 theory ARMv8_Syntax
-  imports ARMv8_Rules
+  imports ARMv8_Rules ARMv8_Inter
 begin
 
 datatype register = r\<^sub>0 | r\<^sub>1 | r\<^sub>2 | r\<^sub>3 | r\<^sub>4 | r\<^sub>5
@@ -56,17 +56,17 @@ definition Z ::  "'b \<Rightarrow> ((nat,'b) bexp)"
   where "Z r = Exp\<^sub>B (\<lambda>x. x!0 = 0) [Var r]"
 
 syntax
-  "_Load"  :: "'r \<Rightarrow> 'r \<Rightarrow> ('v,'r,'a) com_armv8" ("(_ := [_])" [70, 65] 61)
-  "_LoadC"  :: "'r \<Rightarrow> 'r \<Rightarrow> 'c \<Rightarrow> ('v,'r,'a) com_armv8" ("(_ := [_ + #_])" [70, 65] 61)
-  "_LoadIC"  :: "('v,'r,'a) pred \<Rightarrow> 'r \<Rightarrow> 'r \<Rightarrow> 'c \<Rightarrow> ('v,'r,'a) com_armv8" ("(\<lbrace>_\<rbrace> _ := [_ + #_])" [20, 70, 65] 61)
+  "_Load"  :: "'r \<Rightarrow> 'r \<Rightarrow> 'v set \<Rightarrow> ('v,'r,'a) com_armv8" ("(_ := [_]~_)" [70, 65] 61)
+  "_LoadC"  :: "'r \<Rightarrow> 'r \<Rightarrow> 'v set \<Rightarrow> 'c \<Rightarrow> ('v,'r,'a) com_armv8" ("(_ := [_ + #_]~_)" [70, 65] 61)
+  "_LoadIC"  :: "('v,'r,'a) pred \<Rightarrow> 'r \<Rightarrow> 'r \<Rightarrow> 'v set \<Rightarrow> 'c \<Rightarrow> ('v,'r,'a) com_armv8" ("(\<lbrace>_\<rbrace> _ := [_ + #_]~_)" [20, 70, 65] 61)
 
-  "_Store" :: "'r \<Rightarrow> 'r \<Rightarrow> ('v,'r,'a) com_armv8" ("([_] := _)" [70, 65] 61)
-  "_StoreI" :: "('v,'r,'a) pred \<Rightarrow> 'r \<Rightarrow> 'v \<Rightarrow> 'r \<Rightarrow> ('v,'r,'a) com_armv8" ("(\<lbrace>_\<rbrace> [_ + #_] := _)" [20, 70, 65] 61)
-  "_StoreIA" :: "('v,'r,'a) pred \<Rightarrow> 'r \<Rightarrow> 'v \<Rightarrow> 'r \<Rightarrow> ('v,'r,'a) auxfn  \<Rightarrow> ('v,'r,'a) com_armv8" ("(\<lbrace>_\<rbrace> [_ + #_] := _ :\<^sub>a _)" [20, 70, 65] 61)
+  "_Store" :: "'r \<Rightarrow> 'r \<Rightarrow> 'v set \<Rightarrow> ('v,'r,'a) com_armv8" ("([_] := _ ~ _)" [70, 65] 61)
+  "_StoreI" :: "('v,'r,'a) pred \<Rightarrow> 'r \<Rightarrow> 'v \<Rightarrow> 'r \<Rightarrow> 'v set \<Rightarrow> ('v,'r,'a) com_armv8" ("(\<lbrace>_\<rbrace> [_ + #_] := _ ~ _)" [20, 70, 65] 61)
+  "_StoreIA" :: "('v,'r,'a) pred \<Rightarrow> 'r \<Rightarrow> 'v \<Rightarrow> 'r \<Rightarrow> 'v set \<Rightarrow> ('v,'r,'a) auxfn  \<Rightarrow> ('v,'r,'a) com_armv8" ("(\<lbrace>_\<rbrace> [_ + #_] := _ ~ _ :\<^sub>a _)" [20, 70, 65] 61)
   
   "_Fence" :: "(nat,'b,'a) com_armv8" ("(fence)" 61)
   "_CFence" :: "(nat,'b,'a) com_armv8" ("(cfence)" 61)
-  "_Cas" :: "('v,'r,'a) pred \<Rightarrow> 'r \<Rightarrow> 'r \<Rightarrow> 'r \<Rightarrow> 'r \<Rightarrow> ('v,'r,'a) auxfn  \<Rightarrow> ('v,'b,'a) com_armv8" ("(\<lbrace>_\<rbrace> _ := cas _ _ _, _)" [20, 70, 65] 61)
+  "_Cas" :: "('v,'r,'a) pred \<Rightarrow> 'r \<Rightarrow> 'r \<Rightarrow> 'r \<Rightarrow> 'r \<Rightarrow> 'v set \<Rightarrow> ('v,'r,'a) auxfn  \<Rightarrow> ('v,'b,'a) com_armv8" ("(\<lbrace>_\<rbrace> _ := cas _ _ _ ~ _, _)" [20, 70, 65] 61)
 
   "_AddI"  :: "'b \<Rightarrow> 'b \<Rightarrow> nat \<Rightarrow> (nat,'b,'a) com_armv8" ("(_ := _ + #_)" [70, 65, 65] 61)
   "_SubI"  :: "'b \<Rightarrow> 'b \<Rightarrow> nat \<Rightarrow> (nat,'b,'a) com_armv8" ("(_ := _ - #_)" [70, 65, 65] 61)
@@ -90,22 +90,22 @@ syntax
 translations
   "\<^sup>ax := a" \<rightharpoonup> "CONST state_rec.more o \<guillemotleft>\<acute>(state_rec.more_update (_update_name x (\<lambda>_. a)))\<guillemotright>"
 
-  "x := [a]" \<rightharpoonup> "CONST Load (CONST UNIV) (CONST Reg a) x (CONST state_rec.more)"
-  "x := [a + #I]" \<rightharpoonup> "CONST Load (CONST UNIV) (CONST Exp (CONST addI I) [CONST Reg a]) x (CONST state_rec.more)"
-  "\<lbrace>P\<rbrace> x := [a + #I]" \<rightharpoonup> "CONST Load \<llangle>P\<rrangle> (CONST Exp (CONST addI I) [CONST Reg a]) x (CONST state_rec.more)"
+  "x := [a]~v" \<rightharpoonup> "CONST Load (CONST UNIV) v (CONST Var a) x (CONST state_rec.more)"
+  "x := [a + #I]~v" \<rightharpoonup> "CONST Load (CONST UNIV) v (CONST Exp (CONST addI I) [CONST Var a]) x (CONST state_rec.more)"
+  "\<lbrace>P\<rbrace> x := [a + #I]~v" \<rightharpoonup> "CONST Load \<llangle>P\<rrangle> v (CONST Exp (CONST addI I) [CONST Var a]) x (CONST state_rec.more)"
 
-  "[a] := r" \<rightharpoonup> "CONST Store (CONST UNIV) (CONST Reg a) r (CONST state_rec.more)"
-  "\<lbrace>P\<rbrace> [a + #I] := x" \<rightharpoonup> "CONST Store \<llangle>P\<rrangle> (CONST Exp (CONST addI I) [CONST Reg a]) x (CONST state_rec.more)"
-  "\<lbrace>P\<rbrace> [ra + #I] := r :\<^sub>a a" \<rightharpoonup> "CONST Store \<llangle>P\<rrangle> (CONST Exp (CONST addI I) [CONST Reg ra]) r a"
+  "[a] := r ~ v" \<rightharpoonup> "CONST Store (CONST UNIV) v (CONST Var a) r (CONST state_rec.more)"
+  "\<lbrace>P\<rbrace> [a + #I] := x ~ v" \<rightharpoonup> "CONST Store \<llangle>P\<rrangle> v (CONST Exp (CONST addI I) [CONST Var a]) x (CONST state_rec.more)"
+  "\<lbrace>P\<rbrace> [ra + #I] := r ~ v :\<^sub>a a" \<rightharpoonup> "CONST Store \<llangle>P\<rrangle> v (CONST Exp (CONST addI I) [CONST Var ra]) r a"
 
-  "\<lbrace>P\<rbrace> r\<^sub>1 := cas r\<^sub>2 r\<^sub>3 r\<^sub>4, a" \<rightharpoonup> "CONST CAS \<llangle>P\<rrangle> r\<^sub>2 r\<^sub>3 r\<^sub>4 r\<^sub>1 1 0 a"
+  "\<lbrace>P\<rbrace> r\<^sub>1 := cas r\<^sub>2 r\<^sub>3 r\<^sub>4 ~ v, a" \<rightharpoonup> "CONST CAS \<llangle>P\<rrangle> v r\<^sub>2 r\<^sub>3 r\<^sub>4 r\<^sub>1 1 0 a"
 
-  "X := Y - #I" \<rightharpoonup> "CONST Op X (CONST Exp (CONST subI I) [CONST Reg Y])"
-  "X := Y + #I" \<rightharpoonup> "CONST Op X (CONST Exp (CONST addI I) [CONST Reg Y])"
-  "X := Y + Z" \<rightharpoonup> "CONST Op X (CONST Exp (CONST addR) [CONST Reg Y, CONST Reg Z])"
-  "X := Y - Z" \<rightharpoonup> "CONST Op X (CONST Exp (CONST subR) [CONST Reg Y, CONST Reg Z])"
-  "X := Y % #I" \<rightharpoonup> "CONST Op X (CONST Exp (CONST modI I) [CONST Reg Y])"
-  "X := Y % Z" \<rightharpoonup> "CONST Op X (CONST Exp (CONST modR) [CONST Reg Y, CONST Reg Z])"
+  "X := Y - #I" \<rightharpoonup> "CONST Op X (CONST Exp (CONST subI I) [CONST Var Y])"
+  "X := Y + #I" \<rightharpoonup> "CONST Op X (CONST Exp (CONST addI I) [CONST Var Y])"
+  "X := Y + Z" \<rightharpoonup> "CONST Op X (CONST Exp (CONST addR) [CONST Var Y, CONST Var Z])"
+  "X := Y - Z" \<rightharpoonup> "CONST Op X (CONST Exp (CONST subR) [CONST Var Y, CONST Var Z])"
+  "X := Y % #I" \<rightharpoonup> "CONST Op X (CONST Exp (CONST modI I) [CONST Var Y])"
+  "X := Y % Z" \<rightharpoonup> "CONST Op X (CONST Exp (CONST modR) [CONST Var Y, CONST Var Z])"
 
   "X := #I" \<rightharpoonup> "CONST Op X (CONST Exp (CONST movI I) [])"
   "fence" \<rightharpoonup> "CONST Fence"
@@ -118,13 +118,10 @@ translations
 definition inv2
   where "inv2 I \<equiv> {(m,m'). m \<in> glb ` I \<longrightarrow> m' \<in> glb ` I}"
 
-definition rif_checks
-  where "rif_checks c R G = True"
-
 fun fn_valid :: "('v::equal,'r::equal,'a) threads \<Rightarrow> bool"
   where 
     "fn_valid [(R,G,I,P,c,Q)] = (stable\<^sub>t R Q \<and> wellformed R G \<and> guar\<^sub>c c (inv2 I \<inter> G) \<and> 
-                                (wellformed R G \<longrightarrow> stable\<^sub>t R Q \<longrightarrow> P \<subseteq> wp R c Q) \<and>
+                                (stable\<^sub>t R Q \<longrightarrow> P \<subseteq> wp (inv2 I \<inter> R) c Q) \<and>
                                 (wellformed R G \<longrightarrow> rif_checks c R G))" |
     "fn_valid _ = undefined"
 
@@ -144,9 +141,9 @@ translations
 syntax
   "_before"  :: "'b \<Rightarrow> 'a" ("\<^sup>1_" [100] 400)
   "_after"   :: "'b \<Rightarrow> 'a" ("\<^sup>2_" [100] 400)
-  "_mem"     :: "nat \<Rightarrow> 'a" ("\<^sup>s[_]")
-  "_mbefore" :: "nat \<Rightarrow> 'a" ("\<^sup>1[_]")
-  "_mafter"  :: "nat \<Rightarrow> 'a" ("\<^sup>2[_]")
+  "_mem"     :: "'g \<Rightarrow> 'a" ("\<^sup>s[_]")
+  "_mbefore" :: "'g \<Rightarrow> 'a" ("\<^sup>1[_]")
+  "_mafter"  :: "'g \<Rightarrow> 'a" ("\<^sup>2[_]")
   "_reg"     :: "'r \<Rightarrow> 'a" ("\<^sup>r_" [100] 1000)
   "_rbefore" :: "'r \<Rightarrow> 'a" ("\<^sup>1\<^sup>r_")
   "_rafer"   :: "'r \<Rightarrow> 'a" ("\<^sup>2\<^sup>r_")
@@ -154,10 +151,13 @@ syntax
   "_abefore" :: "'b \<Rightarrow> 'a" ("\<^sup>1\<^sup>a_" [100] 400)
   "_aafer"   :: "'b \<Rightarrow> 'a" ("\<^sup>2\<^sup>a_" [100] 400)
 
+definition gld :: "('v,'r,'a) state \<Rightarrow> ('v \<Rightarrow> 'v)"
+  where "gld m \<equiv> \<lambda>v. st m (Glb v)"
+
 translations
   "\<^sup>1x" \<rightleftharpoons> "x (\<acute>CONST fst)"
   "\<^sup>2x" \<rightleftharpoons> "x (\<acute>CONST snd)"
-  "\<^sup>s[X]" \<rightleftharpoons> "(\<acute>CONST st) X"
+  "\<^sup>s[X]" \<rightleftharpoons> "(\<acute>CONST gld) X"
   "\<^sup>1[X]" \<rightleftharpoons> "(CONST st (\<acute>CONST fst)) X"
   "\<^sup>2[X]" \<rightleftharpoons> "(CONST st (\<acute>CONST snd)) X"
   "\<^sup>rX" \<rightleftharpoons> "(\<acute>CONST rg) X"
@@ -191,7 +191,7 @@ translations
   "\<^sup>0\<lbrakk>X\<rbrakk>" \<rightleftharpoons> "(CONST st (\<acute>CONST glb)) X"
   "\<^sup>1\<lbrakk>X\<rbrakk>" \<rightleftharpoons> "(CONST st (\<acute>CONST fst)) X"
   "\<^sup>2\<lbrakk>X\<rbrakk>" \<rightleftharpoons> "(CONST st (\<acute>CONST snd)) X"
-  "\<^bold>rX" \<rightleftharpoons> "CONST Var (CONST Reg X)"
+  "\<^bold>rX" \<rightleftharpoons> "CONST Var (CONST Var X)"
   "\<^sup>0\<^bold>rX" \<rightleftharpoons> "(\<acute>CONST rg) X"
   "\<^sup>1\<^bold>rX" \<rightleftharpoons> "(CONST rg (\<acute>CONST fst)) X"
   "\<^sup>2\<^bold>rX" \<rightleftharpoons> "(CONST rg (\<acute>CONST snd)) X"
@@ -240,5 +240,163 @@ lemma [simp]:
 lemma [simp]:
   "UNIV \<subseteq> assert P = P"
   by (auto simp: assert_def)
+
+lemma [simp]:
+  "x(aux: state_rec.more) = x"
+  by (auto simp: aux_upd_def)
+
+lemma [simp]:
+  "st (glb (x(Glb z :=\<^sub>s e))) = (st (glb x))(z := e)"
+  by (auto simp: st_upd_def glb_def)
+
+lemma [simp]:
+  "st (glb (x(aux:f ))) = (st (glb x))"
+  by (auto simp: st_upd_def glb_def)
+
+lemma glb_in [intro!]:
+  assumes "\<exists>l. \<lparr> st = (\<lambda>v. case v of Reg v \<Rightarrow> l v | _ \<Rightarrow> st m v), \<dots> = state_rec.more m \<rparr> \<in> P"
+  shows "glb m \<in> glb ` P"
+proof -
+  obtain l where "\<lparr> st = (\<lambda>v. case v of Reg v \<Rightarrow> l v | _ \<Rightarrow> st m v), \<dots> = state_rec.more m \<rparr> \<in> P"
+    (is "?m \<in> P")
+    using assms by auto
+  hence "glb ?m \<in> glb ` P" by auto
+  moreover have "glb m = glb ?m" by (auto simp: glb_def)
+  ultimately show ?thesis by auto
+qed
+
+lemma  a:
+  "glb x = glb y \<Longrightarrow> st x (Glb e) = st y (Glb e)"
+  unfolding glb_def
+  by (metis state_rec.select_convs(1))
+
+lemma  b:
+  "glb x = glb y \<Longrightarrow> state_rec.more x = state_rec.more y"
+  unfolding glb_def by simp
+
+lemma [simp]:
+  "st (glb x) y = st x (Glb y)"
+  unfolding glb_def by auto
+
+fun chain
+  where "chain [] Q = Q" | "chain (a#xs) Q = chain xs (wpre a Q)"
+declare chain.simps [simp del]
+
+lemma chain_singleI:
+  "wpre a Q = chain [a] Q"
+  unfolding chain.simps by auto
+
+lemma chain_singleI':
+  "stabilize R Q = chain [env R] Q"
+  unfolding chain.simps by auto
+
+lemma chain_lastE:
+  "chain (xs @ [a]) Q = wpre a ( (chain xs Q))"
+  by (induct xs arbitrary: Q) (auto simp: chain.simps)
+
+lemma chain_lastI:
+  "chain [a] (chain xs Q) = chain (xs@[a]) Q"
+  by (induct xs) (auto simp: chain_lastE chain.simps)
+
+lemma chain_merge:
+  "chain l (chain l' Q) = chain (l'@l) Q"
+  by (induct l' arbitrary: Q) (simp add: chain.simps)+
+
+lemma stabilize_mono:
+  "P \<subseteq> Q \<Longrightarrow> stabilize R P  \<subseteq> stabilize R Q"
+  unfolding stabilize_def by auto
+
+lemma pre_mono:
+  "P \<subseteq> Q \<Longrightarrow> wpre a P \<subseteq> wpre a Q"
+  using  stabilize_mono apply (cases a) apply (auto)
+  by blast
+
+lemma chain_mono:
+  "P \<subseteq> Q \<Longrightarrow> chain xs P \<subseteq> chain xs Q"
+  by (induct xs arbitrary: P Q) (auto simp: pre_mono stabilize_mono chain.simps)
+
+lemma chain1_wpre:
+  "P \<subseteq> chain xs (wpre a Q) \<Longrightarrow> P \<subseteq> chain (a#xs) Q"
+  unfolding chain.simps .
+
+lemma chain1_stab:
+  "P \<subseteq> chain xs (stabilize R Q) \<Longrightarrow> P \<subseteq> chain (env R#xs) Q"
+  unfolding chain.simps by auto
+
+lemma chain0:
+  "P \<subseteq> Q \<Longrightarrow> P \<subseteq>  chain [] Q"
+  unfolding chain.simps .
+
+lemma chain_extend:
+  "P \<subseteq> chain xs (Q \<inter> X) \<Longrightarrow> P \<subseteq> chain xs Q"
+  using chain_mono[of "Q \<inter> X" Q] by (auto simp: )
+
+lemma chain_rewrite:
+  "X \<subseteq> Q \<Longrightarrow> P \<subseteq> chain xs X \<Longrightarrow> P \<subseteq> chain xs Q"
+  using chain_mono  by blast
+
+definition str where
+  "str R P \<equiv> if P \<subseteq> stabilize R P then P else UNIV"
+
+lemma str_mono:
+  "Q \<subseteq> P \<Longrightarrow> Q \<subseteq> str R P"
+  unfolding str_def by (auto simp: )
+
+lemma stabilize_univ:
+  "UNIV \<subseteq> stabilize R UNIV"
+  unfolding stabilize_def by auto
+
+lemma stabilize_str:
+  "str R P \<subseteq> stabilize R (str R P)"
+  unfolding str_def stabilize_def by simp
+
+lemma [simp]: "wpre a (P \<inter> Q) = (wpre a P \<inter> wpre a Q)"
+  by (cases a, auto)
+
+lemma chain_inter: "chain l (P \<inter> Q) = (chain l P \<inter> chain l Q)"
+  by (induct l arbitrary: P Q, auto simp: chain.simps)
+
+lemma stable_stabilize:
+  "stable\<^sub>t R Q \<Longrightarrow> Q \<subseteq> stabilize R Q"
+  unfolding stabilize_def stable_def step\<^sub>t_def
+  by auto
+
+lemma strI:
+  "stable\<^sub>t R Q \<Longrightarrow> K \<subseteq> chain l (str R Q) \<Longrightarrow>  K \<subseteq> chain (env R#l) Q"
+  unfolding chain.simps str_def apply simp
+  using stable_stabilize
+  by (metis (mono_tags) chain_rewrite)
+
+lemma envI:
+  "stable\<^sub>t R Q \<Longrightarrow> K \<subseteq> chain l (Q) \<Longrightarrow>  K \<subseteq> chain (env R#l) Q"
+  unfolding chain.simps str_def apply simp
+  using stable_stabilize
+  by (metis (mono_tags) chain_rewrite)
+
+lemma ir_str:
+  "wpre (ir r e) (str R Q) \<supseteq> str R (wpre (ir r e) Q)"
+  apply (auto simp: str_def stabilize_def st_upd_def)
+   apply (subgoal_tac "rg (x\<lparr>st := (st x)(Reg r := ev\<^sub>E (rg m') e)\<rparr>) = rg (m'\<lparr>st := (st m')(Reg r := ev\<^sub>E (rg m') e)\<rparr>)")
+     apply (subgoal_tac "(glb (x\<lparr>st := (st x)(Reg r := ev\<^sub>E (rg m') e)\<rparr>), glb (m'\<lparr>st := (st m')(Reg r := ev\<^sub>E (rg m') e)\<rparr>)) \<in> R")
+     apply blast
+  apply (auto simp: glb_def)[1]
+  unfolding rg_def apply auto[1]
+  done
+
+lemma cm_str:
+  "wpre (cm b) (str R Q) \<supseteq> str R (wpre (cm b) Q)"
+  by (auto simp: str_def stabilize_def st_upd_def)
+
+lemma ncm_str:
+  "wpre (ncm b) (str R Q) \<supseteq> str R (wpre (ncm b) Q)"
+  by (auto simp: str_def stabilize_def st_upd_def)
+
+lemma ign_str:
+  "Q \<subseteq> str R Q"
+  by (auto simp: str_def)
+
+lemma [simp]:
+  "state_rec.more (glb x) = state_rec.more x"
+  unfolding glb_def by auto
 
 end
